p2b

code/ecdsap256/Hacl.Impl.P256.Ext.fst
@@ -25,26 +25,23 @@ open Spec.P256.MontgomeryMultiplication
 #set-options "--z3rlimit 150 --max_fuel 0 --max_ifuel 0" 
 
 
-val point_to_bin: p: point -> result: lbuffer uint8 (size 64) -> tempBuffer: lbuffer uint64 (size 88) ->
+val point_to_bin: p: point -> result: lbuffer uint8 (size 64) ->
   Stack uint64 
-  (requires fun h -> live h p /\ live h result /\ live h tempBuffer /\ disjoint tempBuffer p /\ disjoint p result /\
+  (requires fun h -> live h p /\ live h result /\ disjoint p result /\
     point_x_as_nat h p < prime /\
     point_y_as_nat h p < prime /\
     point_z_as_nat h p < prime)
-  (ensures fun h0 r h1 -> modifies (loc p |+| loc result |+| loc tempBuffer) h0 h1 /\ (
-    let pointD = fromDomainPoint (point_prime_to_coordinates (as_seq h0 p)) in 
-    let pointNormX, pointNormY, pointNormZ = _norm pointD in 
-  
+  (ensures fun h0 r h1 -> modifies (loc result |+| loc p) h0 h1 /\ (
+    let x, y, z = point_prime_to_coordinates (as_seq h0 p) in 
+    if Spec.P256.isPointAtInfinity (x, y, z) then uint_v r = maxint U64 else uint_v r = 0 /\ (
     let oX = gsub result (size 0) (size 32) in 
     let oY = gsub result (size 32) (size 32) in 
 
-    as_seq h1 oX == Lib.ByteSequence.nat_to_bytes_be 32 pointNormX /\ 
-    as_seq h1 oY == Lib.ByteSequence.nat_to_bytes_be 32 pointNormY /\ (
-    if Spec.P256.isPointAtInfinity pointD then uint_v r = maxint U64 else uint_v r = 0)))
+    as_seq h1 oX == Lib.ByteSequence.nat_to_bytes_be 32 x /\ 
+    as_seq h1 oY == Lib.ByteSequence.nat_to_bytes_be 32 y)))
 
 
-let point_to_bin p result tempBuffer = 
-  norm p p tempBuffer;
+let point_to_bin p result = 
   let isPointAtInfinityResult = isPointAtInfinityPrivate p in 
   fromFormPoint p result; 
   isPointAtInfinityResult
